Discrete Math
=============
Problem: For the following function please provide both a recursive and iterative solution for any given input:

f(x) = f(x-1)^3 + f(x-2)^2 + f(x-3)

where f(3) = 3, f(2) = 2, f(1) = 1

Test Data
=========
$test_data = array (1,2,3,4,5,6);

Output
======

Recursive Solution<br>
<ul>
<li>f(1) = 1</li>
<li>f(2) = 2</li>
<li>f(3) = 3</li>
<li>f(4) = 32</li>
<li>f(5) = 32779</li>
<li>f(6) = 35219817466166</li>
</ul>
Iterative Solution
<ul>
<li>f(1) = 1</li>
<li>f(2) = 2</li>
<li>f(3) = 3</li>
<li>f(4) = 32</li>
<li>f(5) = 32779</li>
<li>f(6) = 35219817466166</li>
</ul>

